add heaplang adequacy

src/later.v
@@ -4,7 +4,7 @@ From iris.proofmode Require Import proofmode.
 From iris.itree Require Import itree wpi trace handler.
 From iris.base_logic.lib Require Export fancy_updates.
 From iris.proofmode Require Import proofmode.
-From ITree Require Import ITree.
+From ITree Require Import ITree Eqit.
 
 Variant laterE : Type → Type :=
   | ELater : laterE ().
@@ -98,3 +98,88 @@ Section wpi_later.
   Proof. exact: wpi_later. Qed.
 
 End wpi_later.
+
+Variant later_exhausted : Set := LaterExhausted.
+
+Definition later_ifn_loop {R E} (n : option nat) (t : itree (laterE +' E) R) : itree E ((option nat * itree (laterE +' E) R) + (R + later_exhausted)) :=
+    match observe t with
+    | RetF r => Ret (inr (inl r))
+    | TauF t => Ret (inl (n, t))
+    | VisF (inl1 e) k =>
+        if bool_decide (n = Some 0) then
+          Ret (inr (inr LaterExhausted))
+        else
+          match e in laterE T return (T → _) → _ with
+            ELater => λ k, Ret (inl ((λ x, x - 1) <$> n, k ()))
+          end k
+    | VisF (inr1 e) k => ITree.map (λ x, inl (n, k x)) (trigger e)
+    end.
+
+Definition later_ifn {R E} (n : option nat) (t : itree (laterE +' E) R) : itree E (R + later_exhausted) :=
+  ITree.iter (λ '(n, t), later_ifn_loop n t) (n, t).
+
+Lemma later_ifn_unfold R E n (t : itree (laterE +' E) R) :
+  later_ifn n t ≈ r ← later_ifn_loop n t;
+   match r with
+   | inl nt => later_ifn nt.1 nt.2
+   | inr r => Ret r
+   end.
+Proof. rewrite /later_ifn unfold_iter. f_equiv => -[[??]|//]. by rewrite tau_eutt. Qed.
+
+Section adequacy.
+  Context {R : Type} {E : Type → Type}.
+  Context `{!invGS Σ} {H : iHandler Σ E}.
+
+  Theorem later_adequacy_empty (t : itree (laterE +' E) R) lat Φ n `{!Sequential H}:
+    (lat = Later ↔ is_Some n) →
+    WPi t @ laterH lat ⊕ H; ∅ {{ Φ }} -∗
+    £ (default 0 n) -∗
+    WPi later_ifn n t @ H; ∅ {{ r,
+      match r with
+      | inl r => Φ r
+      | inr _ => ⌜lat = Later⌝
+      end
+    }}.
+  Proof.
+    move => Hlat. iIntros "Hwp". iRevert (n Hlat).
+    iRevert (t Φ) "Hwp". iApply wpi_iter'; first solve_proper.
+    - iIntros "!>" (Φ t) "Hwp". iIntros (n Hlat) "Hlc".
+      rewrite later_ifn_unfold /later_ifn_loop/=. wpi_norm. by iApply wpi_ret'.
+    - iIntros "!>" (Φ t) "Hwp". iIntros (n Hlat) "Hlc".
+      iEval (rewrite later_ifn_unfold /later_ifn_loop/=). wpi_norm/=.
+      iApply wpi_update. iMod "Hwp". iModIntro. by iApply "Hwp".
+    - iIntros "!>" (Φ A [[]|e] k) "HH"; iIntros (n Hlat) "Hlc".
+      + iEval (rewrite later_ifn_unfold /later_ifn_loop/=).
+        case_bool_decide; wpi_norm/=.
+        * iApply wpi_ret'. iMod "HH". admit.
+        * admit.
+      + iEval (rewrite later_ifn_unfold /later_ifn_loop/=).
+        rewrite /ITree.map. wpi_norm/=.
+        iApply wpi_bind. iApply wpi_trigger. iMod "HH". iModIntro.
+        iDestruct (is_seq with "HH") as "HH".
+        iApply (ihandler_mono with "[Hlc]"); last done. 2: by iIntros "!>" (??).
+        iIntros (a) "Hwp".
+        iModIntro. by iApply "Hwp".
+  Admitted.
+
+  (* TODO: can we get this? *)
+  Theorem later_adequacy (t : itree (laterE +' E) R) lat Φ n M `{!Sequential H} :
+    (lat = Later ↔ is_Some n) →
+    WPi t @ laterH lat ⊕ H; M {{ Φ }} -∗
+    £ (default 0 n) -∗
+    WPi later_ifn n t @ H; M {{ r,
+      match r with
+      | inl r => Φ r
+      | inr _ => ⌜lat = Later⌝
+      end
+    }}.
+  Proof.
+    iIntros (?) "Hwp Hlc".
+    rewrite -wpi_clear_mask. iEval (rewrite -wpi_clear_mask).
+    iMod "Hwp". iModIntro.
+    iDestruct (later_adequacy_empty with "Hwp Hlc") as "Hwp"; [done|].
+    iApply wpi_wand; last done. iIntros (r). destruct r.
+    - eauto.
+    - admit.
+  Abort.
+End adequacy.
